cpSTLC/cpSTLCa_Props.v
@@ -6,7 +6,7 @@
    Properties of STLC are based on
    Sofware Foundations, v.4 
   
-   Last Update: Mon, 18 Oct 2016
+   Last Update: Fri, 29 Oct 2016
  %%%%%%%%%%%%%%%%%%%%%%%%%%%%%%%%%%%%%%%%%%%%%%%%%%%%%%%%%%%%%%%%%%% *) 
 
 
@@ -18,4 +18,272 @@
 (* ***************************************************************** *)
 
 
+Add LoadPath "../..".
 
+Require Import ConceptParams.BasicPLDefs.Maps.
+Require Import ConceptParams.BasicPLDefs.Relations.
+
+Require Import ConceptParams.cpSTLC.cpSTLCa_Defs.
+
+Require Import MSets.MSetFacts.
+
+Require Import Coq.Lists.List.
+Import ListNotations.
+Require Import Coq.Bool.Bool.
+
+Require Import Coq.omega.Omega.
+
+
+(* ################################################################# *)
+(** ** Typing *)
+
+(** First of all we want to prove that [ids_are_unique] is correct, 
+    i.e. if it returns true, than there is no duplicates in the list.    
+
+    A bunch of auxiliary lemmas is needed to prove the main theorem.  
+*)
+
+(* We need some facts from sets... *)
+
+Module IdSetFacts := MSetFacts.WFacts IdSet.
+Module IdSetProps := MSetProperties.WProperties IdSet.
+
+Import IdSet.
+Import IdSetFacts.
+
+Lemma add_eq__mem_true : forall (x : id) (s : id_set),
+    ids_mem x (ids_add x s) = true.
+Proof.
+  intros x s. rewrite mem_1.
+  reflexivity.
+  apply add_1. reflexivity.
+Qed.
+
+Lemma add_neq__mem_ignore : forall (x y : id) (s : id_set),
+    x <> y ->
+    ids_mem y (ids_add x s) = ids_mem y s.
+Proof.
+  intros x y s. intros H. 
+  remember (add_neq_iff s H) as Hneq. clear HeqHneq.
+  repeat (rewrite <- IdSet.mem_spec in Hneq). 
+  unfold ids_mem, ids_add in *.
+  destruct (IdSet.mem y s) eqn:Hmem.
+  - apply Hneq. reflexivity.
+  - destruct (IdSet.mem y (ids_add x s)) eqn:Hmem'.
+    apply Hneq in Hmem'. inversion Hmem'.
+    assumption.
+Qed.
+
+Lemma mem_add_false__mem_false : forall (x y : id) (s : id_set),
+    ids_mem y (ids_add x s) = false ->
+    ids_mem y s = false.
+Proof.
+  intros x y s H.
+  rewrite <- not_mem_iff in H.
+  rewrite <- not_mem_iff. intros Hin.
+  apply add_2 with (x := x) in Hin. auto.
+Qed.  
+
+Lemma add_elem_into_eq__eq : forall (s s' : id_set) (x : id),
+    IdSet.Equal s s' ->
+    IdSet.Equal (ids_add x s) (ids_add x s').
+Proof.
+  intros s s' x Heq.
+  unfold Equal. intros y.
+  split; intros Hin;
+    (destruct (beq_idP x y);
+       [subst; rewrite <- mem_spec;
+        apply add_eq__mem_true
+       |remember (add_3 n Hin) as Hyins;
+        apply add_2; apply Heq; assumption]).
+(* 
+add_2: forall (s : t) (x y : elt), In y s -> In y (add x s)
+add_3: forall (s : t) (x y : elt), x <> y -> In y (add x s) -> In y s 
+*)
+Qed.  
+  
+Lemma ids_are_unique_recur__eq_sets_eq : forall (l : list id) (s s' : id_set),
+    IdSet.Equal s s' ->
+    ids_are_unique_recur l s = ids_are_unique_recur l s'.
+Proof.
+  intros l.
+  induction l as [| h l' IHl'];
+    intros s s' Heq.
+  - (* l = nil *)
+    reflexivity.
+  - (* l = h :: l' *)
+    simpl.
+    destruct (ids_mem h s) eqn:Hhs.
+    + (* h in s *)
+      rewrite mem_spec in Hhs.
+      unfold Equal in Heq. apply Heq in Hhs as Hhs'.
+      rewrite <- mem_spec in Hhs'. unfold ids_mem. rewrite -> Hhs'.
+      reflexivity.
+    + (* h not in s' *)
+      rewrite <- not_mem_iff in Hhs.
+      (* unfold Equal in Heq. *)
+      destruct (ids_mem h s') eqn:Hhs'.
+      * rewrite mem_spec in Hhs'. apply Heq in Hhs'.
+        apply Hhs in Hhs'. contradiction.
+      * rewrite <- not_mem_iff in Hhs'.
+        assert (H: Equal (ids_add h s) (ids_add h s'))
+               by (apply add_elem_into_eq__eq; assumption).
+        apply IHl'. assumption.
+Qed.       
+
+Lemma ids_are_unique_recur__set_permute : forall (l : list id) (s : id_set) (x y : id),
+  ids_are_unique_recur l (ids_add x (ids_add y s))
+  = ids_are_unique_recur l (ids_add y (ids_add x s)).
+Proof.
+  intros l s x y.
+  apply ids_are_unique_recur__eq_sets_eq.
+  apply IdSetProps.add_add.
+(*
+IdSetProps.add_add: forall (s : t) (x x' : elt), Equal (add x (add x' s)) (add x' (add x s))
+*) 
+Qed.           
+
+Lemma ids_are_unique_recur_add_true__true : forall (l : list id) (s : id_set) (x : id),
+    ids_are_unique_recur l (ids_add x s) = true -> 
+    ids_are_unique_recur l s = true.
+Proof.
+  intros l. induction l as [| h l' IHl'].
+  - (* l = nil *)
+    intros. reflexivity.
+  - (* l = h :: l' *)
+    intros s x. simpl. 
+    destruct (ids_mem h (ids_add x s)) eqn:Hmem.
+    + intros Hcontra. inversion Hcontra.
+    + rewrite -> ids_are_unique_recur__set_permute.
+      apply mem_add_false__mem_false in Hmem. rewrite -> Hmem.
+      apply IHl'.
+Qed.    
+
+Lemma ids_are_unique_permute : forall (x y : id) (l : list id),
+    ids_are_unique (x :: y :: l) = ids_are_unique (y :: x :: l).
+Proof.
+  intros x y l.
+  destruct (beq_idP x y).
+  - (* x = y *)
+    subst. reflexivity.
+  - (* x <> y *)
+    unfold ids_are_unique. simpl.
+    rewrite ids_are_unique_recur__set_permute.
+    repeat (rewrite add_neq__mem_ignore; simpl).
+    reflexivity. auto. assumption.
+Qed.    
+    
+Lemma ids_are_unique_cons : forall (x : id) (l : list id),
+    ids_are_unique (x :: l) = true ->
+    ids_are_unique l = true.
+Proof.
+  intros x [| h l'].
+  - (* l = nil *)
+    intros []. reflexivity. 
+  - (* l = h :: l' *)
+    (* intros x. *)
+    unfold ids_are_unique in *. 
+    unfold ids_mem, ids_add, ids_empty in *.
+    simpl in *.
+    destruct (beq_idP h x).
+    + (* h = x *)
+      subst h. rewrite -> add_eq__mem_true.
+      intros Hcontra. inversion Hcontra.
+    + (* h <> x *)
+      rewrite -> add_neq__mem_ignore. simpl.
+      intros H. rewrite ids_are_unique_recur__set_permute in H.
+      apply ids_are_unique_recur_add_true__true in H.
+      assumption.
+      apply not_eq_sym; assumption.
+Qed.      
+
+Lemma ids_are_unique_cons__not_in : forall (l : list id) (x : id),
+    ids_are_unique (x :: l) = true ->
+    ~ List.In x l.
+Proof.
+  intros l. induction l as [| h l'].
+  - (* l = nil *)
+    intros x _ H. inversion H. 
+  - (* l = h :: l' *)
+    intros x H Hin.
+    inversion Hin as [Hxh | Hxl'].
+    + (* h = x *)
+      subst. unfold ids_are_unique in H.
+      simpl in H. rewrite -> add_eq__mem_true in H.
+      inversion H.
+    + (* h in l' *)
+      rewrite ids_are_unique_permute in H.
+      apply ids_are_unique_cons in H.
+      apply IHl' in H. apply H in Hxl'. contradiction.
+Qed.            
+
+(** Here is the main [ids_are_unique] correctness theorem: *)
+
+Theorem ids_are_unique__NoDup__correct : forall (l : list id),
+    ids_are_unique l = true -> NoDup l.
+Proof.
+  intros l. induction l as [ | h l' IHl'].
+  - (* l = nil *)
+    intros H. apply NoDup_nil.
+  - (* l = h :: l' *)
+    intros H. apply ids_are_unique_cons in H as H'.
+    apply IHl' in H'.
+    apply NoDup_cons.
+    apply ids_are_unique_cons__not_in in H. assumption.
+    assumption.
+Qed.
+
+
+
+
+(*
+
+Lemma id_set_In__add_permute : forall (x y z : id) (s : id_set),
+    IdSet.In x (ids_add y (ids_add z s)) ->
+    IdSet.In x (ids_add z (ids_add y s)).
+Proof.
+  intros x y z s. intros Hin.
+  apply add_spec in Hin. inversion Hin as [Heq | Hin'].
+  - (* x = y *)
+    subst. apply add_spec. right.
+    apply add_1. reflexivity.
+  - (* x <> y *)
+    apply add_spec in Hin'. inversion Hin' as [Heq | Hin''].
+    + (* x = z *)
+      subst. apply add_1. reflexivity.
+    + (* x <> z *)
+      apply add_spec. right. apply add_spec. right.
+      assumption.
+Qed.
+
+Lemma mem_true__add_permute : forall (x y z : id) (s : id_set),
+    ids_mem x (ids_add y (ids_add z s)) = true
+    -> ids_mem x (ids_add z (ids_add y s)) = true.
+Proof.
+  intros x y z s.
+  repeat (rewrite -> IdSet.mem_spec).
+  apply id_set_In__add_permute.
+Qed.
+
+Lemma mem_add_permute : forall (x y z : id) (s : id_set),
+    ids_mem x (ids_add y (ids_add z s))
+    = ids_mem x (ids_add z (ids_add y s)).
+Proof.
+  intros x y z s.
+  destruct (ids_mem x (ids_add y (ids_add z s))) eqn:Hmem.
+  - (* mem x (add y (add z s)) = true *)
+    symmetry.
+    apply mem_true__add_permute. assumption.
+  - (* mem x (add y (add z s)) = false *)
+    apply not_mem_iff in Hmem. unfold not in Hmem.
+    symmetry. apply not_mem_iff.
+    intros Hin. apply id_set_In__add_permute in Hin.
+    apply Hmem in Hin; inversion Hin.
+Qed.
+
+(** [id_list_to_id_set] builds set from a list of ids. *)
+
+Definition id_list_to_id_set (l : list id) :=
+  fold_left (fun acc x => ids_add x acc) l ids_empty.
+
+*)
