doc-build.sh
@@ -1,0 +1,9 @@
+#!/bin/bash
+
+workdir=$(dirname "$1")
+fname=$(basename "$1")
+
+cd $workdir
+coqdoc -html --no-index $fname
+cd ..
+
